auxiliary rules spec, bool and proofs updated

AuxRulesBoolScript.sml
@@ -1,14 +1,37 @@
 open preamble AuxSpecTheory AuxBoolTheory
-  
+    
 val _ = new_theory "AuxRulesBool";
 
  
+(* EWIN rule *)
+
+val EWIN_Auxiliary_dec_def = Define `
+  EWIN_Auxiliary_dec ((qu,st,l):params) j1 j2 =
+    ∃u t p bl e h bl2.
+      (j1 = NonFinal (u, t, p, bl, bl2, e, h))
+      /\ (j2 = Final e)
+      /\ ((LENGTH e) = st)`;
+
+(* HWIN rule *)
+
+val HWIN_Auxiliary_dec_def = Define `
+  HWIN_Auxiliary_dec ((qu,st,l):params) j1 j2 =
+    ∃u t p bl e h bl2.
+       (j1 = NonFinal (u, t, p, bl, bl2, e, h))
+       /\ (j2 = Final (e++h))
+       /\ (((LENGTH (e ++ h)) <= st) \/ (((LENGTH e) <= st) /\ (NULL h)))`;
+
+
+
 val ELIM_CAND_Auxiliary_dec_def = Define `
   (ELIM_CAND_Auxiliary_dec (c: cand) ((qu,st,l):params) (t: tallies)
                            (p: piles) (p': piles) (bl2: cand list) bl2' 
                            (e: cand list) (h: cand list) h') <=>  
      
-              (NULL bl2)
+              (NULL bl2) 
+          (* /\ (NULL ba) 
+           /\ (NULL bl)
+           /\ (NULL bl') *) 
            /\ (LENGTH (e ++ h) > st) /\ (LENGTH e < st)
            /\ (¬(NULL l)) /\ (ALL_DISTINCT l)
            /\ (list_MEM_dec (h++e) l)
@@ -22,12 +45,15 @@ val ELIM_CAND_Auxiliary_dec_def = Define `
            /\ (h' = equal_except_dec c h)
            /\ (bigger_than_cand c t h)`;
 
+(* /\ (bl2' = c :: bl2) :: this condition must be added to STVs such as Victoria and Tasmania *)
+(* ((NULL bl2) \/ (~ NULL bl2 /\ (NULL (FLAT (get_cand_pile (HD bl2) p))))) *)
 
 val TRANSFER_Auxiliary_dec_def = Define `
   (TRANSFER_Auxiliary_dec ((qu,st,l):params) (t: tallies)
                            (p: piles) (p': piles) (bl: cand list) (bl2: cand list) 
                            (e: cand list) (h: cand list))  ⇔
       (NULL bl2) 
+(*   /\ (NULL ba) *) 
    /\ (LENGTH e < st)
    /\ (list_MEM_dec (h++e) l)
    /\ ALL_DISTINCT (h++e)
@@ -38,11 +64,17 @@ val TRANSFER_Auxiliary_dec_def = Define `
    /\ (ALL_DISTINCT (MAP FST t))
    /\ (less_than_quota qu t h)
    /\ (~ NULL bl)`;
+(* /\
+  (TRANSFER_Auxiliary_dec _ (Final _) _ = F) /\
+  (TRANSFER_Auxiliary_dec _ _ (Final _) = F)`; *)
+(* ((NULL bl2) \/ (~ NULL bl2 /\ (NULL (FLAT (get_cand_pile (HD bl2) p))))) *)
 
 
 val COUNT_Auxiliary_dec_def = Define `
    (COUNT_Auxiliary_dec ((qu, st, l): params) (ba: ballots) (ba': ballots) (t: tallies)
                          (t': tallies) (p: piles) (p': piles) (e: cand list) (h: cand list)) 
+      (* (NonFinal (ba, t, p, bl, bl2, e, h))
+       (NonFinal (ba', t', p', bl', bl2', e', h')) *) ⇔
    
        ALL_DISTINCT (h++e)
     /\ ALL_DISTINCT (MAP FST p)
@@ -58,11 +90,16 @@ val COUNT_Auxiliary_dec_def = Define `
     /\ (~ NULL ba)
     /\ (~ NULL h)
     /\ (NULL ba')`;
+(* /\
+   (COUNT_Auxiliary_dec _ (Final _) _ = F) /\
+   (COUNT_Auxiliary_dec _ _ (Final _) = F)`; *)
 
 
 val ELECT_Auxiliary_dec = Define `
      (ELECT_Auxiliary_dec ((qu,st,l): params) (ba: ballots) (t: tallies)
-                          (p: piles) (p': piles) bl bl' (e: cand list) e' (h: cand list) h' <=>
+                          (p: piles) (p': piles) bl bl' (e: cand list) e' (h: cand list) h'
+       (*    (NonFinal (ba, t, p, bl, bl2, e, h))
+           (NonFinal (ba', t', p', bl', bl2', e',h')) *) <=>
               let (l1 = (DROP (LENGTH bl) bl'))
                  in
                    (SORTED (tally_comparison t) l1)
@@ -86,14 +123,17 @@ val ELECT_Auxiliary_dec = Define `
                 /\ (~ NULL l)
                 /\ ALL_DISTINCT l
                 /\ (bl = TAKE (LENGTH bl) bl') 
+          (*      /\ (bl' = bl ++ l1) *)
                 /\ (Valid_PileTally_dec1 p l) /\ (Valid_PileTally_dec2 p l)
                 /\ (Valid_PileTally_dec1 p' l) /\ (Valid_PileTally_dec2 p' l)
                 /\ (Valid_PileTally_dec1 t l) /\ (Valid_PileTally_dec2 t l)
                 /\ (list_MEM_dec e' l)
                 /\ (list_MEM_dec h l))`;
+(* /\
+     (ELECT_Auxiliary_dec _ (Final _) _ = F) /\
+     (ELECT_Auxiliary_dec _ _ (Final _) = F)`; *)
 
-
-
+  
 val TRANSFER_EXCLUDED_Auxiliary__dec_def = Define `
        TRANSFER_EXCLUDED_Auxiliary_dec ((qu,st,l):params) ba' (t: tallies)
                            (p: piles) (p': piles) (bl2: cand list) bl2'
@@ -101,24 +141,23 @@ val TRANSFER_EXCLUDED_Auxiliary__dec_def = Define `
        case bl2 of
          c :: ls =>
              (case NULL (get_cand_pile c p') of
-                T => (NULL bl2')
-               |_ => (bl2' = bl2))
-          /\ (LENGTH e) < st
-          /\ (list_MEM_dec (h ++ e) l)
-          /\ (ALL_DISTINCT (h ++ e)) /\ (ALL_DISTINCT (MAP FST p'))
-          /\ (Valid_PileTally_dec1 t l) /\ (Valid_PileTally_dec2 t l)
-          /\ (Valid_PileTally_dec1 p l) /\ (Valid_PileTally_dec2 p l)
+	        T => (NULL bl2')
+	       |_ => (bl2' = bl2))
+	  /\ (LENGTH e) < st
+	  /\ (list_MEM_dec (h ++ e) l)
+	  /\ (ALL_DISTINCT (h ++ e)) /\ (ALL_DISTINCT (MAP FST p')) 
+	  /\ (Valid_PileTally_dec1 t l) /\ (Valid_PileTally_dec2 t l)
+	  /\ (Valid_PileTally_dec1 p l) /\ (Valid_PileTally_dec2 p l)
           /\ (Valid_PileTally_dec1 p' l) /\ (Valid_PileTally_dec2 p' l)
           /\ (~ NULL l) /\ (ALL_DISTINCT l)
-          /\ ALL_DISTINCT (MAP FST t)
-          /\ (less_than_quota qu t h)
-          /\ (let xs = ReGroup_Piles (QSORT3 (\x y. (SND x) <= (SND y)) (FLAT (get_cand_pile c p)))
-               in
-                 (ba' = LAST xs) /\ (MEM (c, (TAKE ((LENGTH xs) - 1) xs)) p'))
-          /\ (subpile2_backlog_trans2 [c] p p') /\ (subpile2_backlog_trans2 [c] p' p)
-         | _ => F `;
-
-
+	  /\ ALL_DISTINCT (MAP FST t)
+	  /\ (less_than_quota qu t h)
+	  /\ (let xs = ReGroup_Piles (QSORT3 (\x y. (SND x) <= (SND y)) (FLAT (get_cand_pile c p)))
+	       in
+	         (ba' = LAST xs) /\ (MEM (c, (TAKE ((LENGTH xs) - 1) xs)) p'))
+	  /\ (subpile2_backlog_trans2 [c] p p') /\ (subpile2_backlog_trans2 [c] p' p)
+         | _ => F `; 
+ 
 
 
 val _ = export_theory ();
