AuxRulesSpecScript.sml
@@ -1,5 +1,5 @@
-open preamble AuxSpecTheory
- 
+open preamble AuxSpecTheory AuxBoolTheory
+       
 val _ = new_theory "AuxRulesSpec";
 
 (* The rules *)
@@ -16,6 +16,25 @@ val _ = new_theory "AuxRulesSpec";
        j1 is the judgement before the rule application
        j2 is the judgement after the rule application
 *)
+
+
+(* EWIN rule *)
+
+val EWIN_Auxiliary_def = Define `
+  EWIN_Auxiliary ((qu,st,l):params) j1 j2 =
+    ∃u t p bl e h bl2.
+      (j1 = NonFinal (u, t, p, bl, bl2, e, h))
+      /\ (j2 = Final e)
+      /\ (LENGTH e) = st`;
+
+(* HWIN rule *)
+
+val HWIN__Auxiliary_def = Define `
+  HWIN_Auxiliary ((qu,st,l):params) j1 j2 =
+    ∃u t p bl e h bl2.
+       (j1 = NonFinal (u, t, p, bl, bl2, e, h))
+       /\ (j2 = Final (e++h))
+       /\ (((LENGTH (e ++ h)) <= st) \/ ((LENGTH (e) <= st) /\ (h = [])))`;
 
 
 (* Auxiliary ELIMINATION rule *)
@@ -39,7 +58,11 @@ val ELIM_CAND_Auxiliary_def = Define `
      /\ MEM c h
      /\ (!d. (MEM d h ==> (?x y. (MEM (c,x) t) /\ (MEM (d,y) t) /\ ( x <= y))))
      /\ equal_except c nh h`;
-  
+
+(* I am letting bl2 to have at most one cand in it at any time so no need to
+ \/ ((~ (bl2 = [])) /\ (FLAT (get_cand_pile (HD bl2) p) = []))) *)
+ 
+(*  /\ (bl2' = c :: bl2) :: to be added for Vic and Tasmania *)    
 
 (* Auxiliary TRANSFER rule *)
 
@@ -47,7 +70,9 @@ val TRANSFER_Auxiliary_def = Define `
   TRANSFER_Auxiliary ((qu,st,l):params) (t: tallies)
                            (p: piles) (p': piles) (bl: cand list) (bl2: cand list) 
                            (e: cand list) (h: cand list) <=>
-        (bl2 = [])
+(*    ? nba t p bl e h nbl np.
+     (j1 = NonFinal ([], t, p, bl, [], e, h)) *)
+        (bl2 = []) 
      /\ (bl <> [])
      /\ (LENGTH e < st)
      /\ (!d. MEM d (h++e) ==> MEM d l)
@@ -59,12 +84,18 @@ val TRANSFER_Auxiliary_def = Define `
      /\ ALL_DISTINCT (MAP FST t)
      /\ (!c'. (MEM c' h ==> (?x. MEM (c',x) t /\ ( x < qu))))`;
 
+(*
+\/ ((bl2 <> []) /\ ((FLAT (get_cand_pile (HD bl2) p)) = [])))
+*)
+
 (* Auxiliary COUNT rule *)
 
 val COUNT_Auxiliary_def = Define `
         (COUNT_Auxiliary ((qu, st, l): params) (ba: ballots) (ba': ballots) (t: tallies)
                          (t': tallies) (p: piles) (p': piles) (e: cand list) (h: cand list)) <=> 
 
+(*? ba t nt p np bl bl2 e h.
+          (j1 = NonFinal (ba, t, p, bl, bl2, e, h)) *)
           (!d. MEM d (h++e) ==> MEM d l)
        /\ ALL_DISTINCT (h++e)
        /\ (Valid_PileTally t l)
@@ -113,14 +144,13 @@ val ELECT_Auxiliary_def = Define `
     /\ (!c. MEM c e' ==> MEM c l)
     /\ (!c. MEM c h ==> MEM c l)`;
 
-
-
+                      
 val TRANSFER_EXCLUDED_Auxiliary_def = Define `
        TRANSFER_EXCLUDED_Auxiliary ((qu,st,l):params) ba' (t: tallies)
                            (p: piles) (p': piles) (bl2: cand list) bl2'
                            (e: cand list) (h: cand list) <=>
-      ? bs c.
-        (bl2 = c :: bs)
+      ? bs c. 
+        (bl2 = c :: bs)	
      /\ ((MEM (c, []) p' ==> (bl2' = []))
         /\ (~ MEM (c, []) p' ==> (bl2' = bl2)))
      /\ (LENGTH e < st)
@@ -137,7 +167,32 @@ val TRANSFER_EXCLUDED_Auxiliary_def = Define `
         (!l'. (MEM (d',l') p ==> MEM (d',l') p')) /\ (!l'. (MEM (d',l') p' ==> MEM (d',l') p)))
      /\ ? xs. xs = ReGroup_Piles (QSORT3 (\x y. (SND x) <= (SND y)) (FLAT (get_cand_pile c p)))
         /\ (ba' = LAST xs)
-        /\ MEM (c, TAKE ((LENGTH xs) - 1) xs) p' `;
+	/\ MEM (c, TAKE ((LENGTH xs) - 1) xs) p' `;
+        
+   
+
+
+
+(*
+/\ (get_cand_pile c p' =
+                       TAKE ((LENGTH (get_cand_pile c p)) - 1) (get_cand_pile c p))
+     /\ ba' = LAST (ReGroup_Piles (FLAT (get_cand_pile c p)))`;
+  
+val Merge_def = Define `
+       (Merge [] ys <=> ys)
+    /\ (Merge xs [] <=> xs)
+    /\ (Merge (x0 :: xs) (y0 :: ys) <=> if (SND x0) <= (SND y0) then x0 :: (Merge xs (y0::ys))
+                                        else y0 :: (Merge  (x0:: xs) ys))`;
+
+
+  
+val MergeSort_def = tDefine "MergeSort" `
+       (MergeSort [] <=> [])
+    /\ (MergeSort [x] <=> [x])
+    /\ (MergeSort xs <=> let half = DIV2 (LENGTH xs) in
+                           Merge (MergeSort (TAKE half xs)) (MergeSort (DROP half xs)))`
+WF_REL_TAC `measure (LENGTH)`                           
+  *)  
 
 
 val _ = export_theory ();
